Correctness of the sieve of Eratosthenes

opentheory/examples/gfp-modular.ml
@@ -62,13 +62,13 @@ let num_to_gfp_mult = new_axiom
 
 new_constant ("gfp_exp", `:gfp -> num -> gfp`);;
 
-let gfp_exp_0 = new_axiom
+let gfp_exp_zero = new_axiom
   `!x. gfp_exp x 0 = num_to_gfp 1`;;
 
 let gfp_exp_suc = new_axiom
   `!x n. gfp_exp x (SUC n) = gfp_mult x (gfp_exp x n)`;;
 
-let gfp_exp_def = CONJ gfp_exp_0 gfp_exp_suc;;
+let gfp_exp_def = CONJ gfp_exp_zero gfp_exp_suc;;
 
 new_constant ("gfp_neg", `:gfp -> gfp`);;
 
@@ -311,13 +311,13 @@ let num_to_gfp_mult = new_axiom
 
 new_constant ("gfp_exp", `:gfp -> num -> gfp`);;
 
-let gfp_exp_0 = new_axiom
+let gfp_exp_zero = new_axiom
   `!x. gfp_exp x 0 = num_to_gfp 1`;;
 
 let gfp_exp_suc = new_axiom
   `!x n. gfp_exp x (SUC n) = gfp_mult x (gfp_exp x n)`;;
 
-let gfp_exp_def = CONJ gfp_exp_0 gfp_exp_suc;;
+let gfp_exp_def = CONJ gfp_exp_zero gfp_exp_suc;;
 
 new_constant ("gfp_neg", `:gfp -> gfp`);;
 
