opentheory/examples/prime.ml
@@ -40,15 +40,27 @@ let prime_three = prove
 
 export_thm prime_three;;
 
+let prime_divides_inj = prove
+  (`!p1 p2. prime p1 /\ prime p2 /\ divides p1 p2 ==> p1 = p2`,
+   REPEAT STRIP_TAC THEN
+   MP_TAC (SPEC `p2 : num` prime_def) THEN
+   ASM_REWRITE_TAC [] THEN
+   STRIP_TAC THEN
+   POP_ASSUM (MP_TAC o SPEC `p1 : num`) THEN
+   ASM_REWRITE_TAC [] THEN
+   STRIP_TAC THEN
+   SUBGOAL_THEN `F` CONTR_TAC THEN
+   UNDISCH_TAC `prime p1` THEN
+   ASM_REWRITE_TAC [prime_one]);;
+
+export_thm prime_divides_inj;;
+
 let prime_even = prove
   (`!p. prime p /\ EVEN p ==> p = 2`,
-   GEN_TAC THEN
-   REWRITE_TAC [prime_def; GSYM two_divides] THEN
    REPEAT STRIP_TAC THEN
-   FIRST_X_ASSUM (MP_TAC o SPEC `2`) THEN
-   ASM_REWRITE_TAC [] THEN
-   NUM_REDUCE_TAC THEN
-   MATCH_ACCEPT_TAC EQ_SYM);;
+   MATCH_MP_TAC EQ_SYM THEN
+   MATCH_MP_TAC prime_divides_inj THEN
+   ASM_REWRITE_TAC [prime_two; two_divides]);;
 
 export_thm prime_even;;
 
@@ -151,6 +163,64 @@ let prime_divisor = prove
 
 export_thm prime_divisor;;
 
+let prime_divisor_lt = prove
+  (`!n.
+      prime n <=>
+      ~(n = 0) /\ ~(n = 1) /\ !p. prime p /\ p < n ==> ~divides p n`,
+   GEN_TAC THEN
+   ASM_CASES_TAC `n = 0` THENL
+   [ASM_REWRITE_TAC [prime_zero];
+    ALL_TAC] THEN
+   ASM_REWRITE_TAC [] THEN
+   ASM_CASES_TAC `n = 1` THENL
+   [ASM_REWRITE_TAC [prime_one];
+    ALL_TAC] THEN
+   ASM_REWRITE_TAC [] THEN
+   EQ_TAC THENL
+   [REPEAT STRIP_TAC THEN
+    UNDISCH_TAC `p < (n : num)` THEN
+    REWRITE_TAC [NOT_LT] THEN
+    MATCH_MP_TAC EQ_IMP_LE THEN
+    MATCH_MP_TAC EQ_SYM THEN
+    MATCH_MP_TAC prime_divides_inj THEN
+    ASM_REWRITE_TAC [];
+    STRIP_TAC THEN
+    REWRITE_TAC [prime_def] THEN
+    ASM_REWRITE_TAC [] THEN
+    X_GEN_TAC `m : num` THEN
+    ASM_CASES_TAC `m = 0` THENL
+    [ASM_REWRITE_TAC [zero_divides];
+     ALL_TAC] THEN
+    STRIP_TAC THEN
+    ASM_CASES_TAC `m = 1` THENL
+    [ASM_REWRITE_TAC [];
+     ALL_TAC] THEN
+    ASM_REWRITE_TAC [] THEN
+    MP_TAC (SPEC `m : num` prime_divisor) THEN
+    ASM_REWRITE_TAC [] THEN
+    STRIP_TAC THEN
+    FIRST_X_ASSUM (MP_TAC o SPEC `p : num`) THEN
+    ASM_REWRITE_TAC [] THEN
+    DISCH_THEN (MP_TAC o ONCE_REWRITE_RULE [GSYM CONTRAPOS_THM]) THEN
+    REWRITE_TAC [NOT_LT] THEN
+    ANTS_TAC THENL
+    [MATCH_MP_TAC divides_trans THEN
+     EXISTS_TAC `m : num` THEN
+     ASM_REWRITE_TAC [];
+     ALL_TAC] THEN
+    STRIP_TAC THEN
+    REWRITE_TAC [GSYM LE_ANTISYM] THEN
+    CONJ_TAC THENL
+    [MATCH_MP_TAC divides_le THEN
+     ASM_REWRITE_TAC [];
+     MATCH_MP_TAC LE_TRANS THEN
+     EXISTS_TAC `p : num` THEN
+     ASM_REWRITE_TAC [] THEN
+     MATCH_MP_TAC divides_le THEN
+     ASM_REWRITE_TAC []]]);;
+
+export_thm prime_divisor_lt;;
+
 let large_prime = prove
   (`!n. ?p. n <= p /\ prime p`,
    GEN_TAC THEN
@@ -191,27 +261,178 @@ let large_prime = prove
 export_thm large_prime;;
 
 (* ------------------------------------------------------------------------- *)
-(* The sieve of Eratosthenes.                                                *)
+(* The stream of all primes in order.                                        *)
 (* ------------------------------------------------------------------------- *)
 
-logfile "natural-prime-sieve-def";;
+logfile "natural-prime-stream-def";;
 
-let (primes_mono,snth_primes) =
+let (primes_mono_le,snth_primes) =
   let def = new_specification ["primes"]
               (MATCH_MP num_stream_exists large_prime) in
   CONJ_PAIR def;;
 
-export_thm primes_mono;;
+export_thm primes_mono_le;;
 export_thm snth_primes;;
 
-let primes_def = CONJ primes_mono snth_primes;;
+let primes_def = CONJ primes_mono_le snth_primes;;
 
-let primes_up_to_def = new_definition
+let primes_below_def = new_definition
   `!n.
-     primes_up_to n =
-     stake primes (minimal i. n < snth primes i)`;;
+     primes_below n =
+     stake primes (minimal i. n <= snth primes i)`;;
 
-export_thm primes_up_to_def;;
+export_thm primes_below_def;;
+
+logfile "natural-prime-stream-thm";;
+
+let prime_primes = prove
+  (`!i. prime (snth primes i)`,
+   GEN_TAC THEN
+   REWRITE_TAC [snth_primes] THEN
+   EXISTS_TAC `i : num` THEN
+   REFL_TAC);;
+
+export_thm prime_primes;;
+
+let primes_mono_lt = prove
+  (`!i j. snth primes i < snth primes j <=> i < j`,
+   REWRITE_TAC [GSYM MONO_LE_LT] THEN
+   ACCEPT_TAC primes_mono_le);;
+
+export_thm primes_mono_lt;;
+
+let primes_mono_le_imp = prove
+  (`!i j. i <= j ==> snth primes i <= snth primes j`,
+   REWRITE_TAC [primes_mono_le]);;
+
+export_thm primes_mono_le;;
+
+let primes_mono_lt_imp = prove
+  (`!i j. i < j ==> snth primes i < snth primes j`,
+   REWRITE_TAC [primes_mono_lt]);;
+
+export_thm primes_mono_le;;
+
+let snth_primes_zero = prove
+  (`snth primes 0 = 2`,
+   REWRITE_TAC [GSYM LE_ANTISYM] THEN
+   CONJ_TAC THENL
+   [STRIP_ASSUME_TAC (REWRITE_RULE [snth_primes] prime_two) THEN
+    POP_ASSUM (SUBST1_TAC o SYM) THEN
+    REWRITE_TAC [primes_mono_le; LE_0];
+    REWRITE_TAC [GSYM NOT_LT; TWO; ONE; LT] THEN
+    MP_TAC (SPEC `0` prime_primes) THEN
+    SPEC_TAC (`snth primes 0`, `n : num`) THEN
+    REPEAT STRIP_TAC THEN
+    FIRST_X_ASSUM SUBST_VAR_TAC THEN
+    POP_ASSUM MP_TAC THEN
+    REWRITE_TAC [GSYM ONE; prime_zero; prime_one]]);;
+
+export_thm snth_primes_zero;;
+
+let primes_below_zero = prove
+  (`primes_below 0 = []`,
+   REWRITE_TAC [primes_below_def; LE_0; MINIMAL_T; stake_zero]);;
+
+export_thm primes_below_zero;;
+
+let primes_below_suc = prove
+  (`!n.
+      primes_below (SUC n) =
+      APPEND (primes_below n) (if prime n then [n] else [])`,
+   GEN_TAC THEN
+   REWRITE_TAC [primes_below_def] THEN
+   COND_CASES_TAC THENL
+   [POP_ASSUM (STRIP_ASSUME_TAC o REWRITE_RULE [snth_primes]) THEN
+    SUBGOAL_THEN
+      `(minimal i. SUC n <= snth primes i) = SUC i` SUBST1_TAC THENL
+    [REWRITE_TAC [LE_SUC_LT] THEN
+     FIRST_X_ASSUM (fun th -> REWRITE_TAC [GSYM th; primes_mono_lt]) THEN
+     MATCH_MP_TAC MINIMAL_EQ THEN
+     REWRITE_TAC [SUC_LT] THEN
+     REWRITE_TAC [LT_SUC_LE; NOT_LT];
+     ALL_TAC] THEN
+    SUBGOAL_THEN
+      `(minimal i. n <= snth primes i) = i` SUBST1_TAC THENL
+    [FIRST_X_ASSUM (fun th -> REWRITE_TAC [GSYM th; primes_mono_le]) THEN
+     MATCH_MP_TAC MINIMAL_EQ THEN
+     REWRITE_TAC [LE_REFL; NOT_LE];
+     ALL_TAC] THEN
+    POP_ASSUM (SUBST1_TAC o SYM) THEN
+    MATCH_ACCEPT_TAC stake_suc';
+    REWRITE_TAC [APPEND_NIL] THEN
+    AP_TERM_TAC THEN
+    AP_TERM_TAC THEN
+    ABS_TAC THEN
+    REWRITE_TAC [LE_SUC_LT] THEN
+    CONV_TAC (LAND_CONV (REWR_CONV LT_LE)) THEN
+    MATCH_MP_TAC (TAUT `!x y. y ==> (x /\ y <=> x)`) THEN
+    STRIP_TAC THEN
+    UNDISCH_TAC `~prime n` THEN
+    ASM_REWRITE_TAC [prime_primes]]);;
+
+export_thm primes_below_suc;;
+
+let primes_below_one = prove
+  (`primes_below 1 = []`,
+   REWRITE_TAC [ONE; primes_below_suc; primes_below_zero] THEN
+   REWRITE_TAC [NIL_APPEND; prime_zero]);;
+
+export_thm primes_below_one;;
+
+let primes_below_two = prove
+  (`primes_below 2 = []`,
+   REWRITE_TAC [TWO; primes_below_suc; primes_below_one] THEN
+   REWRITE_TAC [NIL_APPEND; prime_one]);;
+
+export_thm primes_below_two;;
+
+let primes_below_three = prove
+  (`primes_below 3 = [2]`,
+   REWRITE_TAC [THREE; primes_below_suc; primes_below_two] THEN
+   REWRITE_TAC [NIL_APPEND; prime_two]);;
+
+export_thm primes_below_three;;
+
+let mem_primes_below = prove
+  (`!n p. MEM p (primes_below n) <=> prime p /\ p < n`,
+   REPEAT GEN_TAC THEN
+   SPEC_TAC (`n : num`, `n : num`) THEN
+   INDUCT_TAC THENL
+   [REWRITE_TAC [primes_below_zero; LT; MEM];
+    REWRITE_TAC [LT_SUC_LE] THEN
+    REWRITE_TAC [LE_LT; LEFT_OR_DISTRIB] THEN
+    REWRITE_TAC [primes_below_suc] THEN
+    ASM_REWRITE_TAC [MEM_APPEND] THEN
+    POP_ASSUM (K ALL_TAC) THEN
+    AP_TERM_TAC THEN
+    COND_CASES_TAC THENL
+    [REWRITE_TAC [MEM] THEN
+     ASM_CASES_TAC `p = (n : num)` THEN
+     ASM_REWRITE_TAC [];
+     REWRITE_TAC [MEM] THEN
+     ASM_CASES_TAC `p = (n : num)` THEN
+     ASM_REWRITE_TAC []]]);;
+
+export_thm mem_primes_below;;
+
+let primes_below_divides = prove
+  (`!n.
+      prime n <=>
+      ~(n = 0) /\ ~(n = 1) /\ ALL (\p. ~divides p n) (primes_below n)`,
+   GEN_TAC THEN
+   ONCE_REWRITE_TAC [prime_divisor_lt] THEN
+   AP_TERM_TAC THEN
+   AP_TERM_TAC THEN
+   REWRITE_TAC [GSYM ALL_MEM; mem_primes_below]);;
+
+export_thm primes_below_divides;;
+
+(* ------------------------------------------------------------------------- *)
+(* The sieve of Eratosthenes.                                                *)
+(* ------------------------------------------------------------------------- *)
+
+logfile "natural-prime-sieve-def";;
 
 let (sieve_induct,sieve_recursion) =
   let (induct,recursion) = define_type
@@ -231,10 +452,10 @@ let (sieve_induct,sieve_recursion) =
 export_thm sieve_induct;;
 export_thm sieve_recursion;;
 
-let max_sieve_def = new_recursive_definition sieve_recursion
-  `!n ps. max_sieve (Sieve n ps) = n`;;
+let init_sieve_def = new_definition
+  `init_sieve = Sieve 1 []`;;
 
-export_thm max_sieve_def;;
+export_thm init_sieve_def;;
 
 let max_sieve_def = new_recursive_definition sieve_recursion
   `!n ps. max_sieve (Sieve n ps) = n`;;
@@ -254,7 +475,7 @@ let (inc_counters_sieve_nil,inc_counters_sieve_cons) =
         let (p,(k,j)) = pkj in
         let k' = (k + i) MOD p in
         let j' = j + i in
-        if k' = 0 then (F, CONS (p,(k',j')) ps) else
+        if k' = 0 then (F, CONS (p,(0,j')) ps) else
         let (b,ps') = inc_counters_sieve n j' ps in
         (b, CONS (p,(k',0)) ps'))` in
   let (nil,cons) = CONJ_PAIR def in
@@ -263,7 +484,7 @@ let (inc_counters_sieve_nil,inc_counters_sieve_cons) =
         inc_counters_sieve n i (CONS (p,(k,j)) ps) =
         let k' = (k + i) MOD p in
         let j' = j + i in
-        if k' = 0 then (F, CONS (p,(k',j')) ps) else
+        if k' = 0 then (F, CONS (p,(0,j')) ps) else
         let (b,ps') = inc_counters_sieve n j' ps in
         (b, CONS (p,(k',0)) ps')`,
      REPEAT GEN_TAC THEN
@@ -286,118 +507,440 @@ let inc_sieve_def = new_recursive_definition sieve_recursion
 
 export_thm inc_sieve_def;;
 
-let (inv_counters_sieve_nil,inv_counters_sieve_cons) =
+let (invariant_counters_sieve_nil,invariant_counters_sieve_cons) =
   let def = new_recursive_definition list_RECURSION
-    `(!n i. inv_counters_sieve n i [] <=> T) /\
+    `(!n i. invariant_counters_sieve n i [] <=> T) /\
      (!n i pkj ps.
-        inv_counters_sieve n i (CONS pkj ps) <=>
+        invariant_counters_sieve n i (CONS pkj ps) <=>
         let (p,(k,j)) = pkj in
-        ((k + i) MOD p = n MOD p /\
-         inv_counters_sieve n (i + j) ps))` in
+        (~(p = 0) /\
+         (k + i) MOD p = n MOD p /\
+         invariant_counters_sieve n (i + j) ps))` in
   let (nil,cons) = CONJ_PAIR def in
   let nil' = REWRITE_RULE [] nil in
   let cons' = prove
     (`!n i p k j ps.
-        inv_counters_sieve n i (CONS (p,(k,j)) ps) <=>
+        invariant_counters_sieve n i (CONS (p,(k,j)) ps) <=>
+        ~(p = 0) /\
         (k + i) MOD p = n MOD p /\
-        inv_counters_sieve n (i + j) ps`,
+        invariant_counters_sieve n (i + j) ps`,
      REPEAT GEN_TAC THEN
      CONV_TAC (LAND_CONV (REWR_CONV cons)) THEN
      REWRITE_TAC [LET_DEF; LET_END_DEF]) in
   (nil',cons');;
 
-export_thm inv_counters_sieve_nil;;
-export_thm inv_counters_sieve_cons;;
+export_thm invariant_counters_sieve_nil;;
+export_thm invariant_counters_sieve_cons;;
 
-let inv_counters_sieve_def =
-    CONJ inv_counters_sieve_nil inv_counters_sieve_cons;;
+let invariant_counters_sieve_def =
+    CONJ invariant_counters_sieve_nil invariant_counters_sieve_cons;;
 
-let inv_sieve_def = new_recursive_definition sieve_recursion
+let invariant_sieve_def = new_recursive_definition sieve_recursion
   `!n ps.
-     inv_sieve (Sieve n ps) <=>
+     invariant_sieve (Sieve n ps) <=>
      ~(n = 0) /\
-     MAP FST ps = primes_up_to n /\
-     inv_counters_sieve n 0 ps`;;
+     MAP FST ps = primes_below (n + 1) /\
+     invariant_counters_sieve n 0 ps`;;
 
-export_thm inv_sieve_def;;
+export_thm invariant_sieve_def;;
+
+let next_sieve_exists = prove
+ (`?fn. !s.
+     fn s =
+     let (b,s') = inc_sieve s in
+     if b then (max_sieve s', s')
+     else fn s'`,
+  MP_TAC
+   (ISPECL
+      [`\s : sieve.
+          let (b,s') = inc_sieve s in
+          ~b`;
+       `\s : sieve.
+          let (b,s') = inc_sieve s in
+          s'`;
+       `\s : sieve.
+          let (b,s') = inc_sieve s in
+          (max_sieve s', s')`] WF_REC_TAIL) THEN
+  DISCH_THEN
+    (X_CHOOSE_THEN `fn : sieve -> num # sieve`
+     STRIP_ASSUME_TAC) THEN
+  EXISTS_TAC `fn : sieve -> num # sieve` THEN
+  GEN_TAC THEN
+  FIRST_X_ASSUM (fun th -> CONV_TAC (LAND_CONV (ONCE_REWRITE_CONV [th]))) THEN
+  REWRITE_TAC [] THEN
+  PAIR_CASES_TAC `inc_sieve s` THEN
+  DISCH_THEN
+    (X_CHOOSE_THEN `b : bool`
+        (X_CHOOSE_THEN `s' : sieve` ASSUME_TAC)) THEN
+  ASM_REWRITE_TAC [LET_DEF; LET_END_DEF] THEN
+  BOOL_CASES_TAC `b : bool` THEN
+  REWRITE_TAC []);;
+
+let next_sieve_def =
+  new_specification ["next_sieve"] next_sieve_exists;;
+
+export_thm next_sieve_def;;
 
 logfile "natural-prime-sieve-thm";;
 
-let prime_primes = prove
-  (`!i. prime (snth primes i)`,
-   GEN_TAC THEN
-   REWRITE_TAC [snth_primes] THEN
-   EXISTS_TAC `i : num` THEN
-   REFL_TAC);;
+let sieve_cases = prove_cases_thm sieve_induct;;
 
-export_thm prime_primes;;
+export_thm sieve_cases;;
 
-let snth_primes_0 = prove
-  (`snth primes 0 = 2`,
-   CHOOSE_THEN MP_TAC (REWRITE_RULE [snth_primes] prime_two) THEN
-   NUM_CASES_TAC `i : num` THENL
-   [DISCH_THEN SUBST1_TAC THEN
-    REWRITE_TAC [];
-    ALL_TAC] THEN
-   DISCH_THEN (CHOOSE_THEN SUBST1_TAC) THEN
-   STRIP_TAC THEN
-   SUBGOAL_THEN `F` CONTR_TAC THEN
-   MP_TAC (SPECL [`0`; `SUC n`] primes_mono) THEN
-   ASM_REWRITE_TAC [LT_0; NOT_LT] THEN
-   POP_ASSUM (K ALL_TAC) THEN
-   MP_TAC (SPEC `0` prime_primes) THEN
-   SPEC_TAC (`snth primes 0`, `n : num`) THEN
-   GEN_TAC THEN
-   NUM_CASES_TAC `n : num` THENL
-   [DISCH_THEN SUBST1_TAC THEN
-    REWRITE_TAC [prime_zero];
-    ALL_TAC] THEN
-   DISCH_THEN (X_CHOOSE_THEN `m : num` SUBST1_TAC) THEN
-   REWRITE_TAC [TWO; LE_SUC] THEN
-   NUM_CASES_TAC `m : num` THENL
-   [DISCH_THEN SUBST1_TAC THEN
-    REWRITE_TAC [GSYM ONE; prime_one];
-    ALL_TAC] THEN
-   DISCH_THEN (X_CHOOSE_THEN `n : num` SUBST1_TAC) THEN
-   REWRITE_TAC [ONE; LE_SUC; LE_0]);;
+let sieve_cases_tac = CASES_TAC sieve_cases;;
 
-export_thm snth_primes_0;;
+let sieve_inj = prove_constructors_injective sieve_recursion;;
 
-let primes_up_to_0 = prove
-  (`primes_up_to 0 = []`,
-   REWRITE_TAC [primes_up_to_def] THEN
-   SUBGOAL_THEN `(minimal i. 0 < snth primes i) = 0`
-     (fun th -> REWRITE_TAC [th; stake_0]) THEN
-   MATCH_MP_TAC MINIMAL_EQ THEN
-   REWRITE_TAC [LT; snth_primes_0] THEN
-   NUM_REDUCE_TAC);;
+export_thm sieve_inj;;
 
-export_thm primes_up_to_0;;
-
-(***
-let primes_up_to_suc = prove
-  (`!n.
-      primes_up_to (SUC n) =
-      APPEND (primes_up_to n) (if prime (SUC n) then [SUC n] else [])`,
-   GEN_TAC THEN
-   REWRITE_TAC [primes_up_to_def] THEN
-   COND_CASES_TAC THENL
-   [POP_ASSUM (STRIP_ASSUME_TAC o REWRITE_RULE [snth_primes]) THEN
-    STRIP_
-
-let primes_up_to_1 = prove
-  (`primes_up_to 1 = []`,
-   REWRITE_TAC [primes_up_to_def] THEN
-   SUBGOAL_THEN `(minimal i. 0 < snth primes i) = 0`
-     (fun th -> REWRITE_TAC [th; stake_0]) THEN
-   MATCH_MP_TAC MINIMAL_EQ THEN
-   REWRITE_TAC [LT; snth_primes_0] THEN
-   NUM_REDUCE_TAC);;
-
-let inv_init_sieve = prove
-  (`inv_sieve init_sieve`,
+let invariant_init_sieve = prove
+  (`invariant_sieve init_sieve`,
    REWRITE_TAC
-     [inv_sieve_def; init_sieve_def; inv_counters_sieve_def]
-***)
+     [invariant_sieve_def; init_sieve_def; invariant_counters_sieve_def;
+      ONE; ADD_CLAUSES; MAP; NOT_SUC] THEN
+   REWRITE_TAC [GSYM ONE; GSYM TWO; primes_below_two]);;
+
+export_thm invariant_init_sieve;;
+
+let invariant_counters_sieve_suc = prove
+  (`!n i ps.
+      invariant_counters_sieve (SUC n) (SUC i) ps <=>
+      invariant_counters_sieve n i ps`,
+   REPEAT GEN_TAC THEN
+   SPEC_TAC (`i : num`, `i : num`) THEN
+   SPEC_TAC (`ps : (num # (num # num)) list`,
+             `ps : (num # (num # num)) list`) THEN
+   LIST_INDUCT_TAC THENL
+   [REWRITE_TAC [invariant_counters_sieve_def];
+    ALL_TAC] THEN
+   GEN_TAC THEN
+   PAIR_CASES_TAC `h : num # (num # num)` THEN
+   DISCH_THEN
+     (X_CHOOSE_THEN `p : num`
+        (X_CHOOSE_THEN `kj : num # num` SUBST1_TAC)) THEN
+   PAIR_CASES_TAC `kj : num # num` THEN
+   DISCH_THEN
+     (X_CHOOSE_THEN `k : num`
+        (X_CHOOSE_THEN `j : num` SUBST1_TAC)) THEN
+   ASM_REWRITE_TAC [invariant_counters_sieve_def; ADD_CLAUSES] THEN
+   POP_ASSUM (K ALL_TAC) THEN
+   ASM_CASES_TAC `p = 0` THENL
+   [ASM_REWRITE_TAC [];
+    ALL_TAC] THEN
+   ASM_REWRITE_TAC [] THEN
+   AP_THM_TAC THEN
+   AP_TERM_TAC THEN
+   MATCH_MP_TAC SUC_INJ_MOD THEN
+   FIRST_ASSUM ACCEPT_TAC);;
+
+let invariant_inc_counters_sieve = prove
+  (`!n i ps b ps'.
+      invariant_counters_sieve n i ps /\
+      inc_counters_sieve (SUC n) (SUC i) ps = (b,ps') ==>
+      invariant_counters_sieve (SUC n) 0 ps' /\
+      (b <=> ALL (\ (p,(k,j)). ~divides p (SUC n)) ps) /\
+      (MAP FST ps' = APPEND (MAP FST ps) (if b then [SUC n] else []))`,
+   GEN_TAC THEN
+   ONCE_REWRITE_TAC [SWAP_FORALL_THM] THEN
+   LIST_INDUCT_TAC THENL
+   [REPEAT GEN_TAC THEN
+    REWRITE_TAC
+      [inc_counters_sieve_def; PAIR_EQ; invariant_counters_sieve_def;
+       ALL; MAP; APPEND] THEN
+    STRIP_TAC THEN
+    FIRST_X_ASSUM SUBST_VAR_TAC THEN
+    ASM_REWRITE_TAC [invariant_counters_sieve_def; MAP; ADD_0] THEN
+    MP_TAC (SPEC `SUC n` MOD_REFL) THEN
+    REWRITE_TAC [NOT_SUC] THEN
+    DISCH_THEN SUBST1_TAC THEN
+    MATCH_MP_TAC MOD_0 THEN
+    MATCH_ACCEPT_TAC NOT_SUC;
+    ALL_TAC] THEN
+   REPEAT GEN_TAC THEN
+   PAIR_CASES_TAC `h : num # (num # num)` THEN
+   DISCH_THEN
+     (X_CHOOSE_THEN `p : num`
+        (X_CHOOSE_THEN `kj : num # num` SUBST1_TAC)) THEN
+   PAIR_CASES_TAC `kj : num # num` THEN
+   DISCH_THEN
+     (X_CHOOSE_THEN `k : num`
+        (X_CHOOSE_THEN `j : num` SUBST1_TAC)) THEN
+   REWRITE_TAC
+     [inc_counters_sieve_def; invariant_counters_sieve_def;
+      LET_DEF; LET_END_DEF; ALL] THEN
+   STRIP_TAC THEN
+   POP_ASSUM MP_TAC THEN
+   SUBGOAL_THEN `(k + SUC i) MOD p = SUC n MOD p` SUBST1_TAC THENL
+   [REWRITE_TAC [ADD_CLAUSES] THEN
+    REWRITE_TAC [ADD1] THEN
+    MP_TAC (SPEC `p : num` MOD_ADD_MOD') THEN
+    ASM_REWRITE_TAC [] THEN
+    DISCH_THEN (fun th -> ONCE_REWRITE_TAC [GSYM th]) THEN
+    ASM_REWRITE_TAC [];
+    ALL_TAC] THEN
+   MP_TAC (SPECL [`p : num`; `SUC n`] divides_mod) THEN
+   ASM_REWRITE_TAC [] THEN
+   DISCH_THEN SUBST1_TAC THEN
+   SUBGOAL_THEN `j + SUC i = SUC (i + j)` SUBST1_TAC THENL
+   [REWRITE_TAC [ADD_CLAUSES; SUC_INJ] THEN
+    MATCH_ACCEPT_TAC ADD_SYM;
+    ALL_TAC] THEN
+   COND_CASES_TAC THENL
+   [PURE_REWRITE_TAC [PAIR_EQ] THEN
+    STRIP_TAC THEN
+    FIRST_X_ASSUM SUBST_VAR_TAC THEN
+    FIRST_X_ASSUM (SUBST1_TAC o SYM) THEN
+    REWRITE_TAC [MAP; APPEND_NIL] THEN
+    ASM_REWRITE_TAC
+      [invariant_counters_sieve_def; ADD_CLAUSES;
+       invariant_counters_sieve_suc] THEN
+    MATCH_MP_TAC MOD_0 THEN
+    FIRST_ASSUM ACCEPT_TAC;
+    ALL_TAC] THEN
+   PAIR_CASES_TAC `inc_counters_sieve (SUC n) (SUC (i + j)) t` THEN
+   STRIP_TAC THEN
+   ASM_REWRITE_TAC [PAIR_EQ] THEN
+   STRIP_TAC THEN
+   FIRST_X_ASSUM SUBST_VAR_TAC THEN
+   FIRST_X_ASSUM SUBST_VAR_TAC THEN
+   ASM_REWRITE_TAC
+     [MAP; APPEND; CONS_11; invariant_counters_sieve_def; ADD_0;
+      CONJ_ASSOC'] THEN
+   CONJ_TAC THENL
+   [MATCH_MP_TAC MOD_MOD_REFL THEN
+    FIRST_ASSUM ACCEPT_TAC;
+    ALL_TAC] THEN
+   FIRST_X_ASSUM MATCH_MP_TAC THEN
+   EXISTS_TAC `i + j : num` THEN
+   ASM_REWRITE_TAC []);;
+
+let invariant_inc_sieve = prove
+  (`!s b s'.
+      invariant_sieve s /\
+      inc_sieve s = (b,s') ==>
+      invariant_sieve s' /\
+      max_sieve s' = max_sieve s + 1 /\
+      (b <=> prime (max_sieve s'))`,
+   REPEAT GEN_TAC THEN
+   sieve_cases_tac `s : sieve` THEN
+   STRIP_TAC THEN
+   POP_ASSUM SUBST_VAR_TAC THEN
+   sieve_cases_tac `s' : sieve` THEN
+   STRIP_TAC THEN
+   POP_ASSUM SUBST_VAR_TAC THEN
+   REWRITE_TAC
+     [inc_sieve_def; max_sieve_def; GSYM ADD1; LET_DEF; LET_END_DEF] THEN
+   PAIR_CASES_TAC `inc_counters_sieve (SUC n) 1 ps` THEN
+   STRIP_TAC THEN
+   ASM_REWRITE_TAC [invariant_sieve_def; PAIR_EQ; sieve_inj; GSYM ADD1] THEN
+   STRIP_TAC THEN
+   REPEAT (FIRST_X_ASSUM SUBST_VAR_TAC) THEN
+   REWRITE_TAC [NOT_SUC; CONJ_ASSOC'] THEN
+   MP_TAC
+     (SPECL
+        [`n : num`;
+         `0`;
+         `ps : (num # (num # num)) list`;
+         `b : bool`;
+         `ps' : (num # (num # num)) list`]
+      invariant_inc_counters_sieve) THEN
+   ASM_REWRITE_TAC [GSYM ONE] THEN
+   STRIP_TAC THEN
+   POP_ASSUM SUBST1_TAC THEN
+   SUBGOAL_THEN `b <=> prime (SUC n)` SUBST1_TAC THENL
+   [ASM_REWRITE_TAC [primes_below_divides; NOT_SUC; ONE; SUC_INJ] THEN
+    MATCH_MP_TAC EQ_TRANS THEN
+    EXISTS_TAC
+      `ALL (\p. ~divides p (SUC n))
+         (MAP FST (ps : (num # (num # num)) list))` THEN
+    CONJ_TAC THENL
+    [POP_ASSUM_LIST (K ALL_TAC) THEN
+     REWRITE_TAC [ALL_MAP] THEN
+     AP_THM_TAC THEN
+     AP_TERM_TAC THEN
+     REWRITE_TAC [FUN_EQ_THM] THEN
+     X_GEN_TAC `pkj : num # (num # num)` THEN
+     PAIR_CASES_TAC `pkj : num # (num # num)` THEN
+     DISCH_THEN
+       (X_CHOOSE_THEN `p : num`
+          (X_CHOOSE_THEN `kj : num # num` SUBST1_TAC)) THEN
+     PAIR_CASES_TAC `kj : num # num` THEN
+     DISCH_THEN
+       (X_CHOOSE_THEN `k : num`
+          (X_CHOOSE_THEN `j : num` SUBST1_TAC)) THEN
+     REWRITE_TAC [o_THM];
+     AP_TERM_TAC THEN
+     FIRST_ASSUM ACCEPT_TAC];
+    ALL_TAC] THEN
+   POP_ASSUM (K ALL_TAC) THEN
+   ASM_REWRITE_TAC [] THEN
+   MATCH_MP_TAC EQ_SYM THEN
+   MATCH_ACCEPT_TAC primes_below_suc);;
+
+let invariant_sieve = prove
+  (`!s.
+      invariant_sieve s ==>
+      primes_sieve s = primes_below (max_sieve s + 1)`,
+   GEN_TAC THEN
+   sieve_cases_tac `s : sieve` THEN
+   STRIP_TAC THEN
+   POP_ASSUM SUBST_VAR_TAC THEN
+   REWRITE_TAC [invariant_sieve_def; primes_sieve_def; max_sieve_def] THEN
+   STRIP_TAC);;
+
+export_thm invariant_sieve;;
+
+let invariant_first_sieve = prove
+  (`?s.
+      next_sieve init_sieve = (2,s) /\
+      invariant_sieve s /\
+      max_sieve s = 2`,
+   EXISTS_TAC `Sieve 2 [(2,(0,0))]` THEN
+   ONCE_REWRITE_TAC [next_sieve_def] THEN
+   REWRITE_TAC
+     [inc_sieve_def; init_sieve_def; invariant_sieve_def; max_sieve_def;
+      invariant_counters_sieve_def; MAP; LET_DEF; LET_END_DEF;
+      inc_counters_sieve_def; PAIR_EQ; sieve_inj; CONS_11] THEN
+   NUM_REDUCE_TAC THEN
+   REWRITE_TAC [primes_below_three]);;
+
+let invariant_next_sieve = prove
+  (`!s i n s'.
+      invariant_sieve s /\
+      max_sieve s = snth primes i /\
+      next_sieve s = (n,s') ==>
+      invariant_sieve s' /\
+      n = max_sieve s' /\
+      n = snth primes (SUC i)`,
+   REPEAT GEN_TAC THEN
+   STRIP_TAC THEN
+   POP_ASSUM MP_TAC THEN
+   SUBGOAL_THEN `max_sieve s < snth primes (SUC i)`
+     (CHOOSE_THEN MP_TAC o REWRITE_RULE [LT_EXISTS]) THENL
+   [ASM_REWRITE_TAC [primes_mono_lt; SUC_LT];
+    ALL_TAC] THEN
+   SUBGOAL_THEN `snth primes i <= max_sieve s` MP_TAC THENL
+   [ASM_REWRITE_TAC [LE_REFL];
+    ALL_TAC] THEN
+   POP_ASSUM (K ALL_TAC) THEN
+   POP_ASSUM MP_TAC THEN
+   REWRITE_TAC [IMP_IMP; CONJ_ASSOC'] THEN
+   SPEC_TAC (`s : sieve`, `s : sieve`) THEN
+   SPEC_TAC (`d : num`, `d : num`) THEN
+   INDUCT_TAC THENL
+   [GEN_TAC THEN
+    STRIP_TAC THEN
+    POP_ASSUM MP_TAC THEN
+    ONCE_REWRITE_TAC [next_sieve_def] THEN
+    PAIR_CASES_TAC `inc_sieve s` THEN
+    DISCH_THEN
+      (X_CHOOSE_THEN `b : bool`
+         (X_CHOOSE_THEN `s'' : sieve` ASSUME_TAC)) THEN
+    ASM_REWRITE_TAC [LET_DEF; LET_END_DEF] THEN
+    MP_TAC
+      (SPECL
+         [`s : sieve`;
+          `b : bool`;
+          `s'' : sieve`]
+         invariant_inc_sieve) THEN
+    ASM_REWRITE_TAC [] THEN
+    STRIP_TAC THEN
+    FIRST_X_ASSUM SUBST_VAR_TAC THEN
+    SUBGOAL_THEN `prime (max_sieve s'') <=> T` SUBST1_TAC THENL
+    [REWRITE_TAC [snth_primes] THEN
+     EXISTS_TAC `SUC i` THEN
+     ASM_REWRITE_TAC [] THEN
+     REWRITE_TAC [GSYM ADD1; ADD_CLAUSES];
+     ALL_TAC] THEN
+    REWRITE_TAC [PAIR_EQ] THEN
+    STRIP_TAC THEN
+    FIRST_X_ASSUM SUBST_VAR_TAC THEN
+    FIRST_X_ASSUM SUBST_VAR_TAC THEN
+    ASM_REWRITE_TAC [] THEN
+    REWRITE_TAC [GSYM ADD1; ADD_CLAUSES];
+    ALL_TAC] THEN
+   GEN_TAC THEN
+   STRIP_TAC THEN
+   FIRST_X_ASSUM MATCH_MP_TAC THEN
+   PAIR_CASES_TAC `inc_sieve s` THEN
+   DISCH_THEN
+     (X_CHOOSE_THEN `b : bool`
+        (X_CHOOSE_THEN `s'' : sieve` ASSUME_TAC)) THEN
+   EXISTS_TAC `s'' : sieve` THEN
+   UNDISCH_TAC `next_sieve s = n,s'` THEN
+   DISCH_THEN (MP_TAC o ONCE_REWRITE_RULE [next_sieve_def]) THEN
+   ASM_REWRITE_TAC [LET_DEF; LET_END_DEF] THEN
+   MP_TAC
+     (SPECL
+        [`s : sieve`;
+         `b : bool`;
+         `s'' : sieve`]
+        invariant_inc_sieve) THEN
+   ASM_REWRITE_TAC [] THEN
+   STRIP_TAC THEN
+   FIRST_X_ASSUM SUBST_VAR_TAC THEN
+   SUBGOAL_THEN `prime (max_sieve s'') <=> F` SUBST1_TAC THENL
+   [ASM_REWRITE_TAC [snth_primes] THEN
+    DISCH_THEN (X_CHOOSE_THEN `j : num` STRIP_ASSUME_TAC) THEN
+    MP_TAC (SPEC `i < (j : num)` EXCLUDED_MIDDLE) THEN
+    REWRITE_TAC [DE_MORGAN_THM] THEN
+    REWRITE_TAC [NOT_LT; GSYM LT_SUC_LE] THEN
+    ONCE_REWRITE_TAC [GSYM primes_mono_lt] THEN
+    ASM_REWRITE_TAC [LT_ADD_LCANCEL] THEN
+    REWRITE_TAC [ONE; LT_SUC; LT_0; ADD_CLAUSES] THEN
+    ASM_REWRITE_TAC [LT_SUC_LE];
+    ALL_TAC] THEN
+   REWRITE_TAC [PAIR_EQ] THEN
+   STRIP_TAC THEN
+   ASM_REWRITE_TAC [] THEN
+   REWRITE_TAC [GSYM ADD1; ADD_CLAUSES] THEN
+   MATCH_MP_TAC LT_IMP_LE THEN
+   ASM_REWRITE_TAC [LT_SUC_LE]);;
+
+let correct_sieve = prove
+  (`sunfold next_sieve init_sieve = primes`,
+   MATCH_MP_TAC snth_eq_imp THEN
+   GEN_TAC THEN
+   ONCE_REWRITE_TAC [sunfold] THEN
+   MP_TAC invariant_first_sieve THEN
+   STRIP_TAC THEN
+   ASM_REWRITE_TAC [LET_DEF; LET_END_DEF] THEN
+   POP_ASSUM MP_TAC THEN
+   POP_ASSUM MP_TAC THEN
+   POP_ASSUM (K ALL_TAC) THEN
+   REWRITE_TAC [GSYM snth_primes_zero] THEN
+   CHOOSE_THEN SUBST1_TAC (REWRITE_RULE [LE_EXISTS] (SPEC `n : num` LE_0)) THEN
+   REWRITE_TAC [IMP_IMP; CONJ_ASSOC'] THEN
+   CONV_TAC (RAND_CONV (LAND_CONV (RAND_CONV (REWR_CONV ZERO_ADD)))) THEN
+   SPEC_TAC (`0`, `i : num`) THEN
+   SPEC_TAC (`s : sieve`, `s : sieve`) THEN
+   SPEC_TAC (`d : num`, `d : num`) THEN
+   INDUCT_TAC THENL
+   [REPEAT STRIP_TAC THEN
+    REWRITE_TAC [snth_scons_zero; ADD_0];
+    ALL_TAC] THEN
+   REPEAT STRIP_TAC THEN
+   REWRITE_TAC [snth_scons_suc] THEN
+   REWRITE_TAC [ADD_SUC; GSYM SUC_ADD] THEN
+   ONCE_REWRITE_TAC [sunfold] THEN
+   PAIR_CASES_TAC `next_sieve s` THEN
+   DISCH_THEN
+     (X_CHOOSE_THEN `n : num`
+        (X_CHOOSE_THEN `s' : sieve` ASSUME_TAC)) THEN
+   ASM_REWRITE_TAC [LET_DEF; LET_END_DEF] THEN
+   MP_TAC
+     (SPECL
+        [`s : sieve`;
+         `i : num`;
+         `n : num`;
+         `s' : sieve`]
+        invariant_next_sieve) THEN
+   ASM_REWRITE_TAC [] THEN
+   STRIP_TAC THEN
+   POP_ASSUM SUBST_VAR_TAC THEN
+   FIRST_X_ASSUM MATCH_MP_TAC THEN
+   ASM_REWRITE_TAC []);;
+
+export_thm correct_sieve;;
 
 logfile_end ();;
